Finished up assembly correctness

13AssemblyCode/Assemble.thy
@@ -7,7 +7,7 @@ primrec assemble_op_len :: "byte_code \<Rightarrow> nat" where
 | "assemble_op_len (BPushCon k) = 8"
 | "assemble_op_len (BPushLam pc) = 12"
 | "assemble_op_len BApply = 24"
-| "assemble_op_len BReturn = 3"
+| "assemble_op_len BReturn = 4"
 | "assemble_op_len BJump = 21"
 
 primrec assemble_op :: "(nat \<Rightarrow> nat) \<Rightarrow> byte_code \<Rightarrow> assm list" where
@@ -72,6 +72,7 @@ primrec assemble_op :: "(nat \<Rightarrow> nat) \<Rightarrow> byte_code \<Righta
     ASub Vals 1]"
 | "assemble_op mp BReturn = [
     AJmp,
+    APut Stk Stk (Con 0),
     AGet Acc Stk Stk,
     ASub Stk 2]"
 | "assemble_op mp BJump = [
@@ -111,19 +112,19 @@ definition assemble_code :: "byte_code list \<Rightarrow> assm list" where
 definition assemble_heap :: "nat \<Rightarrow> (nat \<Rightarrow> nat) \<Rightarrow> (nat \<Rightarrow> nat) \<Rightarrow> nat \<Rightarrow> nat" where
   "assemble_heap hp mp h x = (if x < hp \<and> x mod 3 = 2 \<and> h (x - 2) = 0 then mp (h x) else h x)"
 
-definition assemble_stack :: "(nat \<Rightarrow> nat) \<Rightarrow> (nat \<Rightarrow> nat) \<Rightarrow> nat \<Rightarrow> nat" where
-  "assemble_stack mp s x = (if even x then mp (s x) else s x)"
+definition assemble_stack :: "nat \<Rightarrow> (nat \<Rightarrow> nat) \<Rightarrow> (nat \<Rightarrow> nat) \<Rightarrow> nat \<Rightarrow> nat" where
+  "assemble_stack sp mp s x = (if x < sp \<and> even x then mp (s x) else s x)"
 
 primrec assemble_state :: "(nat \<Rightarrow> nat) \<Rightarrow> unstr_state \<Rightarrow> assm_state" where
   "assemble_state mp (US h hp e ep vs vp sh sp pc) = 
-    AS (case_register (assemble_heap hp mp h) e vs (assemble_stack mp sh) nmem nmem) 
+    AS (case_register (assemble_heap hp mp h) e vs (assemble_stack sp mp sh) nmem nmem) 
       (case_register hp ep vp sp 0 0) (mp pc)"
 
 abbreviation assm_hp :: "nat \<Rightarrow> byte_code list \<Rightarrow> (nat \<Rightarrow> nat) \<Rightarrow> nat \<Rightarrow> nat" where
   "assm_hp hp cd \<equiv> assemble_heap hp (assembly_map cd)"
 
-abbreviation assm_stk :: "byte_code list \<Rightarrow> (nat \<Rightarrow> nat) \<Rightarrow> nat \<Rightarrow> nat" where
-  "assm_stk cd \<equiv> assemble_stack (assembly_map cd)"
+abbreviation assm_stk :: "nat \<Rightarrow> byte_code list \<Rightarrow> (nat \<Rightarrow> nat) \<Rightarrow> nat \<Rightarrow> nat" where
+  "assm_stk sp cd \<equiv> assemble_stack sp (assembly_map cd)"
 
 abbreviation assm_state :: "byte_code list \<Rightarrow> unstr_state \<Rightarrow> assm_state" where
   "assm_state cd \<equiv> assemble_state (assembly_map cd)"
@@ -160,7 +161,7 @@ lemma [simp]: "assembly_map cd (length cd) = length (assemble_code cd)"
 lemma [simp]: "assm_hp hp cd nmem = nmem"
   by (auto simp add: assemble_heap_def)
 
-lemma [simp]: "assm_stk cd nmem = nmem"
+lemma [simp]: "assm_stk 0 cd m = m"
   by (auto simp add: assemble_stack_def)
 
 lemma assemble_code_lookup' [simp]: "cd ! pc = op \<Longrightarrow> pc < length cd \<Longrightarrow> 
@@ -310,27 +311,31 @@ lemma [simp]: "h (vs vp) = Suc x \<Longrightarrow>
     assemble_heap hp mp h (Suc (Suc (vs vp))) = h (Suc (Suc (vs vp)))"
   by (simp add: assemble_heap_def)
 
-lemma [simp]: "even sp \<Longrightarrow> assm_stk cd sh (Suc sp) = sh (Suc sp)"
+lemma [simp]: "even sp \<Longrightarrow> assm_stk (Suc (Suc sp)) cd sh (Suc sp) = sh (Suc sp)"
   by (simp add: assemble_stack_def)
 
-lemma [simp]: "even sp \<Longrightarrow> ((assm_stk cd sh)(sp := assembly_map cd pc, Suc sp := a)) = 
-    (assm_stk cd (sh(sp := pc, Suc sp := a)))"
+lemma [simp]: "even sp \<Longrightarrow> ((assm_stk sp cd sh)(sp := assembly_map cd pc, Suc sp := a)) = 
+    (assm_stk (Suc (Suc sp)) cd (sh(sp := pc, Suc sp := a)))"
   by (auto simp add: assemble_stack_def)
 
 lemma [simp]: "even (Suc sp) \<Longrightarrow> 
-    (assm_stk cd sh)(sp := Suc (Suc ep)) = assm_stk cd (sh(sp := Suc (Suc ep)))"
+    (assm_stk (Suc sp) cd sh)(sp := Suc (Suc ep)) = assm_stk (Suc sp) cd (sh(sp := Suc (Suc ep)))"
   by (auto simp add: assemble_stack_def)
 
-lemma [simp]: "even (Suc sp) \<Longrightarrow> assm_stk cd sh sp = sh sp"
+lemma [simp]: "even (Suc (Suc sp)) \<Longrightarrow> 
+    ((assm_stk (Suc (Suc sp)) cd sh)(sp := 0)) = assm_stk sp cd (sh(sp := 0))"
+  by rule (auto simp add: assemble_stack_def)
+
+lemma [simp]: "even (Suc sp) \<Longrightarrow> assm_stk (Suc sp) cd sh sp = sh sp"
   by (simp add: assemble_stack_def)
 
-lemma [simp]: "even (Suc (Suc sp)) \<Longrightarrow> assm_stk cd sh sp = assembly_map cd (sh sp)"
+lemma [simp]: "even (Suc (Suc sp)) \<Longrightarrow> assm_stk (Suc (Suc sp)) cd sh sp = assembly_map cd (sh sp)"
   by (simp add: assemble_stack_def)
 
-lemma [simp]: "odd sp \<Longrightarrow> (assm_stk cd sh)(sp := sh sp) = assm_stk cd sh"
+lemma [simp]: "odd sp \<Longrightarrow> (assm_stk (Suc sp) cd sh)(sp := sh sp) = assm_stk sp cd sh"
   by (auto simp add: assemble_stack_def)
 
-lemma [simp]: "assm_stk cd (sh(0 := 0, Suc 0 := 0)) = ((assm_stk cd sh)(0 := 0, Suc 0 := 0))"
+lemma [simp]: "assm_stk 2 cd (sh(0 := 0, Suc 0 := 0)) = (sh(0 := 0, Suc 0 := 0))"
   by (auto simp add: assemble_stack_def)
 
 lemma [simp]: "x < y \<Longrightarrow> (concat (replicate y [a, b]) @ bs) ! (2 * x) = a"
@@ -392,21 +397,21 @@ proof (induction cd\<^sub>b \<Sigma>\<^sub>u \<Sigma>\<^sub>u' rule: evalu.induc
   moreover from evu_lookup have "assemble_code cd ! (5 + 2 * x + assembly_map cd pc) = 
     AGet Acc Stk Acc" by (simp add: nth_append)
   ultimately have "iter_evala (assemble_code cd) 3 
-    (AS (case_register (assm_hp hp cd h) e vs (assm_stk cd sh) nmem nmem) 
+    (AS (case_register (assm_hp hp cd h) e vs (assm_stk (Suc sp) cd sh) nmem nmem) 
       (case_register hp ep vp (Suc sp) 0 0) (8 + 2 * x + assembly_map cd pc)) = 
-        Some (AS (case_register (assm_hp hp cd h) e vs (assm_stk cd sh) nmem nmem) 
+        Some (AS (case_register (assm_hp hp cd h) e vs (assm_stk (Suc sp) cd sh) nmem nmem) 
           (case_register hp ep vp (Suc sp) (sh sp) 0) (5 + 2 * x + assembly_map cd pc))" 
     by (simp add: numeral_def)
   moreover from evu_lookup have "iter_evala (assemble_code cd) (5 + 2 * x) 
-    (AS (case_register (assm_hp hp cd h) e vs (assm_stk cd sh) nmem nmem) 
+    (AS (case_register (assm_hp hp cd h) e vs (assm_stk (Suc sp) cd sh) nmem nmem) 
       (case_register hp ep vp (Suc sp) (sh sp) 0) (5 + 2 * x + assembly_map cd pc)) = 
-        Some (AS (case_register (assm_hp hp cd h) e (vs(vp := y)) (assm_stk cd sh) nmem nmem) 
-          (case_register hp ep (Suc vp) (Suc sp) 0 0) (assembly_map cd pc))" by simp
+        Some (AS (case_register (assm_hp hp cd h) e (vs(vp := y)) (assm_stk (Suc sp) cd sh) 
+          nmem nmem) (case_register hp ep (Suc vp) (Suc sp) 0 0) (assembly_map cd pc))" by simp
   ultimately have "iter_evala (assemble_code cd) (3 + (5 + 2 * x)) 
-    (AS (case_register (assm_hp hp cd h) e vs (assm_stk cd sh) nmem nmem) 
+    (AS (case_register (assm_hp hp cd h) e vs (assm_stk (Suc sp) cd sh) nmem nmem) 
       (case_register hp ep vp (Suc sp) 0 0) (8 + 2 * x + assembly_map cd pc)) = 
-        Some (AS (case_register (assm_hp hp cd h) e (vs(vp := y)) (assm_stk cd sh) nmem nmem)
-          (case_register hp ep (Suc vp) (Suc sp) 0 0) (assembly_map cd pc))" 
+        Some (AS (case_register (assm_hp hp cd h) e (vs(vp := y)) (assm_stk (Suc sp) cd sh) 
+          nmem nmem) (case_register hp ep (Suc vp) (Suc sp) 0 0) (assembly_map cd pc))" 
     using iter_evala_combine by blast
   with evu_lookup show ?case by auto
 next
@@ -422,10 +427,10 @@ next
   moreover from evu_pushcon have "assemble_code cd ! (2 + assembly_map cd pc) = AAdd Hp 1"
     by (simp del: add_2_eq_Suc) 
   ultimately have "iter_evala (assemble_code cd) 8 (AS (case_register (assm_hp hp cd h) e vs 
-    (assm_stk cd sh) nmem nmem) (case_register hp ep vp (Suc sp) 0 0) (assembly_map cd (Suc pc))) = 
-      Some (AS (case_register (assm_hp (3 + hp) cd (h(hp := 1, Suc hp := k, Suc (Suc hp) := 0))) e 
-        (vs(vp := hp)) (assm_stk cd sh) nmem nmem) (case_register (3 + hp) ep (Suc vp) (Suc sp) 0 0)
-          (assembly_map cd pc))" 
+    (assm_stk (Suc sp) cd sh) nmem nmem) (case_register hp ep vp (Suc sp) 0 0) 
+      (assembly_map cd (Suc pc))) = Some (AS (case_register (assm_hp (3 + hp) cd (h(hp := 1,
+        Suc hp := k, Suc (Suc hp) := 0))) e (vs(vp := hp)) (assm_stk (Suc sp) cd sh) nmem nmem) 
+          (case_register (3 + hp) ep (Suc vp) (Suc sp) 0 0) (assembly_map cd pc))" 
     by (auto simp add: numeral_def)
   thus ?case by auto
 next
@@ -448,10 +453,10 @@ next
   moreover from evu_pushlam have "assemble_code cd ! (2 + assembly_map cd pc) = AMov Acc (Con 0)" 
     by (simp del: add_2_eq_Suc) 
   ultimately have "iter_evala (assemble_code cd) 12 (AS (case_register (assm_hp hp cd h) e vs 
-    (assm_stk cd sh) nmem nmem) (case_register hp ep vp (Suc sp) 0 0) (assembly_map cd (Suc pc))) = 
-      Some (AS (case_register (assm_hp (3 + hp) cd (h(hp := 0, Suc hp := sh sp, 
-        Suc (Suc hp) := pc'))) e (vs(vp := hp)) (assm_stk cd sh) nmem nmem) (case_register (3 + hp) 
-          ep (Suc vp) (Suc sp) 0 0) (assembly_map cd pc))" 
+    (assm_stk (Suc sp) cd sh) nmem nmem) (case_register hp ep vp (Suc sp) 0 0) 
+      (assembly_map cd (Suc pc))) = Some (AS (case_register (assm_hp (3 + hp) cd (h(hp := 0, 
+        Suc hp := sh sp, Suc (Suc hp) := pc'))) e (vs(vp := hp)) (assm_stk (Suc sp) cd sh) 
+          nmem nmem) (case_register (3 + hp) ep (Suc vp) (Suc sp) 0 0) (assembly_map cd pc))" 
     by (auto simp add: numeral_def)
   thus ?case by auto
 next
@@ -491,21 +496,23 @@ next
   moreover from evu_apply have "assemble_code cd ! (2 + assembly_map cd pc) = AAdd Acc 1" 
     by (simp del: add_2_eq_Suc)
   ultimately have "iter_evala (assemble_code cd) 24 (AS (case_register (assm_hp hp cd h) e vs 
-    (assm_stk cd sh) nmem nmem) (case_register hp ep (Suc (Suc vp)) (Suc sp) 0 0) 
+    (assm_stk (Suc sp) cd sh) nmem nmem) (case_register hp ep (Suc (Suc vp)) (Suc sp) 0 0) 
       (assembly_map cd (Suc pc))) = Some (AS (case_register (assm_hp hp cd h) 
-        (e(ep := vs (Suc vp), Suc ep := h (Suc (vs vp)))) vs (assm_stk cd (sh(Suc sp := pc, 
-          Suc (Suc sp) := Suc (Suc ep)))) nmem nmem) (case_register hp (Suc (Suc ep)) vp 
-            (Suc (Suc (Suc sp))) 0 0) (assembly_map cd (h (Suc (Suc (vs vp))))))" 
+        (e(ep := vs (Suc vp), Suc ep := h (Suc (vs vp)))) vs (assm_stk (Suc (Suc (Suc sp))) cd 
+          (sh(Suc sp := pc, Suc (Suc sp) := Suc (Suc ep)))) nmem nmem) (case_register hp 
+            (Suc (Suc ep)) vp (Suc (Suc (Suc sp))) 0 0) (assembly_map cd (h (Suc (Suc (vs vp))))))" 
     by (auto simp add: numeral_def)
   thus ?case by auto
 next
   case (evu_return cd pc h hp e ep vs vp sh sp)
-  moreover from evu_return have "assemble_code cd ! (2 + assembly_map cd pc) = ASub Stk 2" 
+  moreover from evu_return have "assemble_code cd ! (3 + assembly_map cd pc) = ASub Stk 2" by simp
+  moreover from evu_return have "assemble_code cd ! (2 + assembly_map cd pc) = AGet Acc Stk Stk" 
     by (simp del: add_2_eq_Suc)
-  ultimately have "iter_evala (assemble_code cd) 3 (AS (case_register (assm_hp hp cd h) e vs 
-    (assm_stk cd sh) nmem nmem) (case_register hp ep vp (Suc (Suc sp)) 0 0) 
-      (assembly_map cd (Suc pc))) = Some (AS (case_register (assm_hp hp cd h) e vs (assm_stk cd sh)
-        nmem nmem) (case_register hp ep vp sp 0 0) (assembly_map cd (sh sp)))" 
+  ultimately have "iter_evala (assemble_code cd) 4 (AS (case_register (assm_hp hp cd h) e vs 
+    (assm_stk (Suc (Suc sp)) cd sh) nmem nmem) (case_register hp ep vp (Suc (Suc sp)) 0 0)
+      (assembly_map cd (Suc pc))) = Some (AS (case_register (assm_hp hp cd h) e vs 
+        (assm_stk sp cd (sh(sp := 0))) nmem nmem) (case_register hp ep vp sp 0 0) 
+          (assembly_map cd (sh sp)))" 
     by (auto simp add: numeral_def)
   thus ?case by auto
 next
@@ -542,10 +549,10 @@ next
   moreover from evu_jump have "assemble_code cd ! (2 + assembly_map cd pc) = AAdd Acc 1" 
     by (simp del: add_2_eq_Suc)
   ultimately have "iter_evala (assemble_code cd) 21 (AS (case_register (assm_hp hp cd h) e vs 
-    (assm_stk cd sh) nmem nmem) (case_register hp ep (Suc (Suc vp)) (Suc sp) 0 0) 
+    (assm_stk (Suc sp) cd sh) nmem nmem) (case_register hp ep (Suc (Suc vp)) (Suc sp) 0 0) 
       (assembly_map cd (Suc pc))) = Some (AS (case_register (assm_hp hp cd h) 
-        (e(ep := vs (Suc vp), Suc ep := h (Suc (vs vp)))) vs (assm_stk cd (sh(sp := Suc (Suc ep)))) 
-          nmem nmem) (case_register hp (Suc (Suc ep)) vp (Suc sp) 0 0)  
+        (e(ep := vs (Suc vp), Suc ep := h (Suc (vs vp)))) vs (assm_stk (Suc sp) cd 
+          (sh(sp := Suc (Suc ep)))) nmem nmem) (case_register hp (Suc (Suc ep)) vp (Suc sp) 0 0)  
             (assembly_map cd (h (Suc (Suc (vs vp))))))" 
     by (auto simp add: numeral_def)
   thus ?case by auto
